Include automatic generation of bosqueTypes.

ref_impl/src/verifier/bosqueTypesFST.ts
@@ -1,0 +1,126 @@
+//-------------------------------------------------------------------------------------------------------
+// Copyright (C) Microsoft. All rights reserved.
+// Licensed under the MIT license. See LICENSE.txt file in the project root for full license information.
+//-------------------------------------------------------------------------------------------------------
+
+import * as FS from "fs";
+
+function printBosqueTypesFST() {
+
+    const fd = FS.openSync("fstar_files/bosqueTypes.fst", 'w');
+
+    const fstar_program = "module BosqueTypes\n \
+    \n \
+    open Sequence\n \
+    module Util=Util\n \
+    \n \
+    // Convention with UnionTerm: \n \
+    // 1) its elements should be unique\n \
+    // 2) There is a unique way to represent any union (normal form)\n \
+    // the latter was needed for eqType\n \
+    type bosqueType =\n \
+    | BAnyType\n \
+    | BSomeType\n \
+    | BTruthyType\n \
+    | BNoneType\n \
+    | BUnionType : bosqueType -> bosqueType -> bosqueType\n \
+    | BParseableType\n \
+    | BBoolType\n \
+    | BIntType\n \
+    | BFloatType // Bad news, FStar doesn't provide support for this type\n \
+    | BRegexType // Bad news, FStar doesn't provide support for this type\n \
+    | BTypedStringType : bosqueType -> bosqueType\n \
+    | BGUIDType\n \
+    // The bool indicates if the Tuple is open or not\n \
+    | BTupleType : bool -> n:nat -> sequence bosqueType n -> bosqueType\n \
+    // FIX: The following is wrong\n \
+    // The bool indicates if the Record is open or not\n \
+    | BRecordType : bool -> n:nat -> sequence bosqueType n -> bosqueType\n \
+    // FIX: The following is incomplete\n \
+    | BFunctionType\n \
+    // FIX: The following is incomplete\n \
+    | BObjectType\n \
+    // FIX: The following is incomplete\n \
+    | BEnumType \n \
+    // FIX: The following is incomplete\n \
+    | BCustomKeyType\n \
+    // FIX: The following is incomplete\n \
+    | BKeyedType\n \
+    | BErrorType\n \
+    // User-defined types\n \
+    | BnSMain__PlayerMarkType\n \
+    | BnSMain__ArtistType\n \
+    | BnSMain__MusicianType\n \
+    \n \
+    (* Definition of equality relation on Bosque types *)\n \
+    val eqTypeSeq : n:nat -> sequence bosqueType n -> sequence bosqueType n -> Tot bool \n \
+    let rec eqTypeSeq n x y = match x with\n \
+    | SNil -> (match y with \n \
+             | SNil -> true\n \
+             | _ -> false\n \
+             )\n \
+    | SCons x1 m xs1 -> (match y with \n \
+                       | SNil -> false\n \
+                       | SCons y1 m' ys1 -> (m = m') && x1 = y1 && eqTypeSeq m xs1 ys1\n \
+                       )\n \
+        \n \
+        (* Definition to encode the subtype relation on Bosque types \n \
+            i.e.forall x y.subtypeOf x y <===> x :> y *) \n \
+        val subtypeOfSeq: n: nat -> x: sequence bosqueType n -> sequence bosqueType n -> Tot bool(decreases x) \n \
+    val subtypeOf: x: bosqueType -> bosqueType -> Tot bool(decreases x) \n \
+    let rec subtypeOf x y = match x, y with\n \
+    | BAnyType, _ -> true\n \
+    | BSomeType, BAnyType -> false\n \
+    | BSomeType, BTruthyType -> false\n \
+    | BSomeType, BNoneType -> false\n \
+    | BSomeType, _ -> true\n \
+    | BTruthyType, BNoneType -> true\n \
+    | BNoneType, BNoneType -> true\n \
+    | BUnionType x1 y1, BUnionType x2 y2 -> (subtypeOf x1 x2 || subtypeOf x1 y2) && (subtypeOf y1 x2 || subtypeOf y1 y2) \n \
+    | BUnionType x1 y1, z -> subtypeOf x1 z || subtypeOf y1 z \n \
+    // | BParseabletype, ? -> ?\n \
+    | BBoolType, BBoolType -> true\n \
+    | BIntType, BIntType -> true\n \
+    // | BFloatType, ? -> ?\n \
+    // | BRegexType, ? -> ?\n \
+    | BTypedStringType t1, BTypedStringType t2 -> subtypeOf t1 t2\n \
+    | BTupleType b1 0 SNil, BTupleType b2 0 SNil -> b1 = b2\n \
+    | BTupleType b1 0 SNil, BTupleType _ _ _ -> b1\n \
+    | BTupleType b1 n1 seq1, BTupleType b2 n2 seq2 -> \n \
+    if b1 then \n \
+    if (n1 > n2) then false\n \
+        else b1 && (n1 <= n2) && subtypeOfSeq n1 seq1(take n2 n1 seq2) \n \
+      else \n \
+    if b2 then false \n \
+        else \n \
+    if (n1 = n2) then(not b1) && (not b2) && (n1 = n2) && subtypeOfSeq n1 seq1 seq2\n \
+          else false \n \
+    // | BRecordType, ? -> ?\n \
+    // | BFunctionType, ? -> ?\n \
+    // | BObjectType, ? -> ?\n \
+    // | BEnumType, ? -> ?\n \
+    // | BCustomType, ? -> ?\n \
+    // | BKeyedType, ? -> ?\n \
+    // User-defined types: TODO: Implement proper subtyping\n \
+    // relations via the provide relation\n \
+    | BnSMain__PlayerMarkType, BnSMain__PlayerMarkType -> true\n \
+    | BnSMain__ArtistType, BnSMain__ArtistType -> true\n \
+    | BnSMain__MusicianType, BnSMain__MusicianType -> true\n \
+    \n \
+    | _, _ -> false\n \
+    and \n \
+    subtypeOfSeq n x y = match x with\n \
+    | SNil -> (match y with\n \
+             | SNil -> true\n \
+             | _ -> false\n \
+             ) \n \
+    | SCons x1 m xs1 -> (match y with \n \
+                       | SNil -> false\n \
+                       | SCons y1 m' ys1 -> (m = m') && (subtypeOf x1 y1) && subtypeOfSeq m xs1 ys1  \n \
+                       ) \n";
+
+    FS.writeSync(fd, fstar_program);
+    FS.closeSync(fd);
+}
+
+export { printBosqueTypesFST }
